moved to functional substitutions; various other cleanups

ModularEngine/src/LogicEngine.FStar/coredkal2.fst
@@ -11,493 +11,365 @@
 // *********************************************************
 *)
 
-(************************************************)
-(* build:                                       *)
-(* fstar typeHeaders.fst types.fst coredkal.fst *)
-(* or:                                          *)
-(* make coredkal                                *)
-(************************************************)
-
 module CoreDKAL
-
-(********************)
-(* Type definitions *)
-(********************)
-
+open TypeHeaders
 open Types
 open Util
-open Typing
 open Subst
+open Typing
+open Unify
 
-val memInfostrate : i:term -> k:infostrate -> b:bool{b=true <=> (In i k)}
-(* impl todo *)
-  
-(******************************)
-(* Trusted external functions *)
-(******************************)
-(* Queries to external databases i.e., Substrate *)
-type SubstrateSays :: substrate => ISubstrateQueryTerm => E
-val check_substrate : s:substrate -> q:ISubstrateQueryTerm -> b:bool{b=true => SubstrateSays s q}
-(* impl todo *)
-
-(***********************)
-(* Inductive judgments *)
-(***********************)
+(*********************************************************************************)
+(* Quotation prefixes *)
+(*********************************************************************************)
 logic function WithPrefix : prefix -> term -> term 
 assume forall (i:term). (WithPrefix [] i) = i
 assume forall (p:term) (pfx:prefix) (i:term). (WithPrefix (p::pfx) i) = (WithPrefix pfx (App SaidInfon [p; i]))
-
-logic function WithPrefixL : prefix -> list term -> list term
-assume forall (pfx:prefix). (WithPrefixL pfx []) = []
-assume forall (pfx:prefix) (t:term) (tl:list term). (WithPrefixL pfx (t::tl)) = ((WithPrefix pfx t)::(WithPrefixL pfx tl))
-assume forall (p:term) (pfx:prefix) (i:term). (WithPrefix (p::pfx) i) = (App SaidInfon [p; (WithPrefix pfx i)])
-
 val withPrefix: pfx:prefix -> i:term -> j:term{j=(WithPrefix pfx i)}
 let rec withPrefix pfx i = match pfx with 
   | [] -> i
   | p::pfx' -> (withPrefix pfx' (App SaidInfon [p; i]))
 
-val stripPrefix: i:term -> pref:prefix -> j:term{(WithPrefix pref j)=i}
-(* stripPrefix is a partial function *)
+(*********************************************************************************)
+(* Alpha conversion (for polyterms in infostrate) *)
+(*********************************************************************************)
+type alphaEquiv :: polyterm => polyterm => P =
+  | AEQ_Mono: i:term -> alphaEquiv (MonoTerm i) (MonoTerm i)
 
-val unify: u:varDecl 
-        -> s1:substitution
-        -> i:term    
-        -> goal:term (* u subsetof (freevars goal) *)
-        -> option (s2:substitution{Extends s2 s1})
-(* ad hoc implementation of unification
-     informally, only variables in u are available for unification.
-*)
+  | AEQ_Poly: 
+       xs:vars -> t:term -> ys:vars 
+    -> polytyping [] (ForallT xs t)
+    -> wfG ys 
+    -> varsTyEq xs ys
+    -> alphaEquiv (ForallT xs t) 
+                  (ForallT ys (Subst t (MkSubst xs (AsTerms ys))))
 
-val allSharedPrefixes : u:varDecl
-                     -> s1:substitution
-                     -> i:term 
-                     -> j:term 
-                     -> list (s2:substitution{Extends s2 s1} * 
-                              pfx2:prefix * 
-                              i':term{Subst i s2 (WithPrefix pfx2 i')}  * 
-                              j':term{Subst j s2 (WithPrefix pfx2 j')})
-(* TODO *)
-
-
-val withPrefixL: pfx:prefix -> i:list term -> j:list term{j=(WithPrefixL pfx i)}
-
-type entails :: substrate => infostrate => varDecl => term => P =
+val alphaConvert: i:polyterm -> (j:polyterm * alphaEquiv i j)
+let alphaConvert i = match i with 
+  | MonoTerm t -> (i, AEQ_Mono t)
+  | ForallT xs t -> 
+      match doPolyTyping [] i with 
+        | MkPartial ityping -> 
+            let ys, pfzip = freshVars xs in
+              match decideWFG ys with 
+                | None -> raise "Impos"
+                | Some wf_ys -> 
+                    let s = mkSubst xs (asTerms ys) in 
+                    let t' = subst t s in 
+                      (ForallT ys t', AEQ_Poly xs t ys ityping wf_ys pfzip)
+  
+(*********************************************************************************)
+(* Definition of DKAL entailment *)
+(*********************************************************************************)
+type entails :: substrate => infostrate => vars => term => P =
   | Entails_Emp : 
-       S:substrate -> K:infostrate -> G:varDecl
+       S:substrate -> K:infostrate -> G:vars
     -> pref:prefix
-    -> WF S K G
-    -> types G (WithPrefix pref (App EmptyInfon [])) Infon
+    -> typing G (WithPrefix pref (App EmptyInfon [])) Infon
     -> entails S K G (WithPrefix pref (App EmptyInfon []))
 
-  | Entails_Hyp_Knowledge : 
-       S:substrate -> K:infostrate -> G:varDecl
-    -> i:term{In i K}
-    -> WF S K G
-    -> entails S K G i
-
-  | Entails_Hyp_Substrate : 
-       S:substrate -> K:infostrate -> G:varDecl
-    -> q:ISubstrateQueryTerm{SubstrateSays S q}     (* Eventually, we get a signature from the DB about this fact *)
-    -> WF S K G
-    -> entails S K G (App AsInfon [(SubstrateQueryTerm q)])
-
-  | Entails_Q_Intro : 
-       S:substrate -> K:infostrate -> G:varDecl
-    -> x:var -> i:term 
-    -> entails S K (x::G) i
-    -> entails S K G (ForallT x i)
-
-  | Entails_Q_Inst : 
-       S:substrate -> K:infostrate -> G:varDecl
-    -> v:var -> i:term -> u:term 
-    -> i':term{Subst i (Update EmptySubst v u) i'}
-    -> entails S K G (ForallT v i)
-    -> types G u v.typ
-    -> entails S K G i'
- 
-  | Entails_And_Intro : 
-       S:substrate -> K:infostrate -> G:varDecl
-    -> ilist:list term -> pref:prefix
-    -> MapL term (entails S K G) (WithPrefixL pref ilist)
-    -> entails S K G (WithPrefix pref (App AndInfon ilist))
-
-  | Entails_And_Intro2 : (* Simpler version with binary And *)
-       S:substrate -> K:infostrate -> G:varDecl
+  | Entails_And_Intro : (* Simpler version with binary And *)
+       S:substrate -> K:infostrate -> G:vars
     -> i:term -> j:term -> pref:prefix
     -> entails S K G (WithPrefix pref i)
     -> entails S K G (WithPrefix pref j)
     -> entails S K G (WithPrefix pref (App AndInfon [i;j]))
-
-  | Entails_And_Elim : (* + well-typedness condition? *)
-       S:substrate -> K:infostrate -> G:varDecl
-    -> ilist:list term -> i:term{In i ilist} -> pref:prefix
-    -> entails S K G (WithPrefix pref (App AndInfon ilist))
-    -> entails S K G (WithPrefix pref i)
     
   | Entails_And_Elim1 : 
-       S:substrate -> K:infostrate -> G:varDecl
+       S:substrate -> K:infostrate -> G:vars
     -> i1:term -> i2:term -> pref:prefix
     -> entails S K G (WithPrefix pref (App AndInfon [i1; i2]))
     -> entails S K G (WithPrefix pref i1)
     
   | Entails_And_Elim2 : 
-       S:substrate -> K:infostrate -> G:varDecl
+       S:substrate -> K:infostrate -> G:vars
     -> i1:term -> i2:term -> pref:prefix
     -> entails S K G (WithPrefix pref (App AndInfon [i1; i2]))
     -> entails S K G (WithPrefix pref i2)
     
   | Entails_W_Imp_Intro : 
-       S:substrate -> K:infostrate -> G:varDecl
+       S:substrate -> K:infostrate -> G:vars
     -> i:term -> j:term -> pref:prefix
     -> entails S K G (WithPrefix pref j)
-    -> types G i Infon
+    -> typing G i Infon
     -> entails S K G (WithPrefix pref (App ImpliesInfon [i; j]))
 
   | Entails_Imp_Elim : 
-       S:substrate -> K:infostrate -> G:varDecl
+       S:substrate -> K:infostrate -> G:vars
     -> i:term -> j:term -> pref:list term
     -> entails S K G (WithPrefix pref i)
     -> entails S K G (WithPrefix pref (App ImpliesInfon [i;j]))
     -> entails S K G (WithPrefix pref j)
 
-  | Entails_Alpha :
-      S:substrate -> K:infostrate -> G:varDecl
-    -> x:var -> i:term -> y:var -> i':term{Subst i (Update EmptySubst x (Var y)) i'}
-    -> entails S K G (ForallT y i')
-    -> entails S K G (ForallT x i)
+  | Entails_Hyp_Substrate :
+       S:substrate -> K:infostrate -> G:vars
+    -> q:ISubstrateQueryTerm{SubstrateSays S q}     (* Eventually, we get a signature from the DB about this fact *)
+    -> entails S K G (App AsInfon [(SubstrateQueryTerm q)])
+
+  | Entails_Q_Elim:
+       S:substrate -> K:infostrate -> G:vars
+    -> xs:vars -> t:term -> is:list term 
+    -> polyentails S K G (ForallT xs t)
+    -> Zip term var (fun (i:term) (x:var) => typing G i x.typ) is xs
+    -> entails S K G (Subst t (MkSubst xs is))
+
+  | Entails_Poly:
+       S:substrate -> K:infostrate -> G:vars
+    -> i:term
+    -> polyentails S K G (MonoTerm i)
+    -> entails S K G i
+
+and polyentails :: substrate => infostrate => vars => polyterm => P = 
+  | Entails_Hyp_Knowledge :
+       S:substrate -> K:infostrate -> G:vars
+    -> i:polyterm{In i K}
+    -> i':polyterm
+    -> polytyping [] i
+    -> alphaEquiv i i'
+    -> polytyping G i'
+    -> polyentails S K G i'
+
+  | Entails_Q_Intro :
+       S:substrate -> K:infostrate -> G:vars
+    -> i:term 
+    -> wfG G
+    -> entails S K G i 
+    -> polyentails S K [] (ForallT G i)
+
+  | Entails_Mono: 
+      S:substrate -> K:infostrate -> G:vars
+    -> i:term
+    -> entails S K G i
+    -> polyentails S K G (MonoTerm i)
 
 (*************************)
-(* Derivation algorithms *)
+(* Derivation algorithm  *)
 (*************************)
-
 (* prove as lemmas *)
-assume forall (s1:substitution) (s2:substitution) (s3:substitution). 
+assume Extends_trans: forall (s1:substitution) (s2:substitution) (s3:substitution). 
             Extends s3 s2 && Extends s2 s1 => Extends s3 s1
-assume forall (pref:prefix) (pref':prefix) (t:term) (t':term) (s:substitution). 
-             (SubstList pref s pref' && Subst t s t')
-            => Subst (WithPrefix pref t) s (WithPrefix pref' t')
+assume Prefix_subst_commute: forall (pref:prefix) (t:term) (s:substitution). 
+          (Subst (WithPrefix pref t) s)=(WithPrefix (SubstList pref s) (Subst t s))
 
-type result :: _ = 
-    (fun (s:substrate) (k:infostrate) (g:varDecl) (s3:substitution) (pref:prefix) (goal:term) => 
-        (goal':term{Subst goal s3 goal'} * pref':prefix{SubstList pref s3 pref'} * entails s k g (WithPrefix pref' goal')))
-        (* (goal':term{Subst goal s4 goal'} * pref':prefix{SubstList pref s4 pref'} * entails s k g (WithPrefix pref' goal'))) *)
+type kresult :: _ = (fun (s:substrate) (k:infostrate) (g:vars) (pref:prefix) (goal:term) (s2:substitution) => 
+    Partial (entails s k g (Subst (WithPrefix pref goal) s2)))
+type kpolyresult :: _ = (fun (s:substrate) (k:infostrate) (g:vars) (goal:polyterm) (s2:substitution) => 
+    Partial (polyentails s k g (PolySubst goal s2)))
 		
 val doDerive:   S:substrate 
              -> K:infostrate 
-             -> G:varDecl
-             -> U:varDecl             (* Variables available for unification in goal *)
+             -> G:vars
+             -> U:vars
              -> s1:substitution
              -> pref:prefix 
              -> goal:term
              -> option (s2:substitution{Extends s2 s1} *
-                          (s3:substitution{Extends s3 s2} ->  (goal':term{Subst goal s3 goal'} *
-                                                                 pref':prefix{SubstList pref s3 pref'} *
-                                                                 entails S K G (WithPrefix pref' goal'))))
-																 
+                          (s3:substitution{Extends s3 s2} -> Partial (entails S K G (Subst (WithPrefix pref goal) s3))))
 
-(* tries to prove (withPrefix pref goal) using (infon);
-   but really what we will eventually prove is
-   (withPrefix pref_infon (withPrefix pref goal))
-   and we really know (withPrefix pref_infon infon)
-*)
-val tryDerive:  S:substrate 
-             -> K:infostrate 
-             -> G:varDecl
-             -> U:varDecl             (* Variables available for unification in goal *)
-             -> s1:substitution
-             -> pref:prefix 
-             -> goal:term
-             -> infon:term
-             -> mkpf_infon:(s4:substitution{Extends s4 s1}
-                             -> (infon':term{Subst infon s4 infon'} *
-                                 entails S K G infon'))
-             -> option (s2:substitution{Extends s2 s1} *
-                          (s3:substitution{Extends s3 s2} 
-                             -> (goal':term{Subst goal s3 goal'} *
-                                 pref':prefix{SubstList pref s3 pref'} *
-                                 entails S K G (WithPrefix pref' goal'))))
-val tryDeriveWrapper:  S:substrate 
-                    -> K:infostrate 
-                    -> G:varDecl
-                    -> U:varDecl             (* Variables available for unification in goal *)
+val tryDeriveAlpha:    S:substrate
+                    -> K:infostrate
+                    -> G:vars
+                    -> U:vars 
                     -> s1:substitution
+                    -> pref:prefix
                     -> goal:term
-                    -> infon:term{In infon K}
+                    -> infon:polyterm{In infon K}
                     -> option (s2:substitution{Extends s2 s1} *
-                                 (s3:substitution{Extends s3 s2} 
-                                  -> (goal':term{Subst goal s3 goal'} *
-                                        entails S K G goal')))
+                                 (s3:substitution{Extends s3 s2} -> Partial (entails S K G (Subst (WithPrefix pref goal) s3))))
 
-let rec tryDerive s k g u s1 pref goal infon mkpf_infon = 
-  match infon with
-  | App AndInfon [infon1; infon2] ->
-      let mkpf_infon1 (s4:substitution{Extends s4 s1}) =
-        let (infon', pf_infon') = mkpf_infon s4 in
-        let infon1' = subst infon1 s4 in (* TODO: inefficient, should grab the one from infon', but need an inversion lemma *)
-        let infon2' = subst infon2 s4 in
-        if infon' = App AndInfon [infon1'; infon2']
-        then ((infon1', Entails_And_Elim1 s k g infon1' infon2' [] pf_infon') :                             
-                (infon1':term{Subst infon1 s4 infon1'} * entails s k g infon1'))
-        else raise "impos" in (* TODO: unreachable, since infon1 and infon2 are q-free (so subst is deterministic) *)
-      (match tryDerive s k g u s1 pref goal infon1 mkpf_infon1 with
-         | Some res -> Some res
-         | None -> 
-            let mkpf_infon2 (s4:substitution{Extends s4 s1}) =
-              let (infon', pf_infon') = mkpf_infon s4 in
-              let infon1' = subst infon1 s4 in
-              let infon2' = subst infon2 s4 in
-              if infon' = App AndInfon [infon1'; infon2']
-              then ((infon2', Entails_And_Elim2 s k g infon1' infon2' [] pf_infon') :                             
-                      (infon2':term{Subst infon2 s4 infon2'} * entails s k g infon2'))
-              else raise "impos" in 
-              tryDerive s k g u s1 pref goal infon1 mkpf_infon1) 
-        
-  | App ImpliesInfon [i; j] ->
-      (match doDerive s k g u s1 [] i with (* for now, []; later change it, cf. suff *)
-         | None -> None
-         | Some((s2, mkpf_i)) ->
-             let mkpf_j (s4:substitution{Extends s4 s2}) =
-               let (i', pref_i', pf_i') = mkpf_i s4 in
-               let (infon', pf_infon') = mkpf_infon s4 in
-               let j' = subst j s4 in
-               if infon' = (App ImpliesInfon [i'; j']) 
-               then ((j', Entails_Imp_Elim s k g i' j' pref_i' pf_i' pf_infon') :
-                       (j':term{Subst j s4 j'} * entails s k g j'))
-               else raise "impos" (* TODO: Unreachable *)
-             in
-               match tryDerive s k g u s2 pref goal j mkpf_j with 
-                 | None -> None 
-                 | Some ((s3, mkpf)) -> Some (s3, mkpf)) (* Need to repack the existential at a different type *)
+val tryDerive:  S:substrate
+             -> K:infostrate
+             -> G:vars
+             -> U:vars
+             -> s1:substitution
+             -> pref:prefix
+             -> goal:term
+             -> infon:polyterm        (* closed polyterm *)
+             -> mkpf_infon:(s4:substitution{Extends s4 s1} -> kpolyresult S K G infon s4)
+             -> option (s2:substitution{Extends s2 s1} *
+                          (s3:substitution{Extends s3 s2} -> Partial (entails S K G (Subst (WithPrefix pref goal) s3))))
 
-  | _ -> 
-      let pref_goal = withPrefix pref goal in
-        match unify u s1 infon pref_goal with 
-          | None -> None
-          | Some s2 -> 
-              let continuation (s3:substitution{Extends s3 s2}) = 
-                let s3_infon, entails_s3_infon = mkpf_infon s3 in 
-                let s3_goal = subst goal s3 in  (* Subst goal s3 s3_goal *)
-                let s3_pref = substList pref s3 in  (* SubstList pref s3 s3_pref *)
-                let s3_pref_goal = withPrefix s3_pref s3_goal in  (* s3_pref_goal = (WithPrefix s3_pref s3_goal) *)
-                  if (s3_pref_goal:term) = s3_infon then 
-                    ((s3_goal, s3_pref, entails_s3_infon) : 
-                       (goal':term{Subst goal s3 goal'} *
-                          pref':prefix{SubstList pref s3 pref'} *
-                          entails s k g (WithPrefix pref' goal')))
-                  else raise "bad substitution" in 
-                Some (s2, continuation) 
-
-and tryDeriveWrapper s k g u s1 goal infon = 
-  let callTryDerive (arg :
-                       (s2:substitution{Extends s2 s1} *
-                          pref:prefix *
-                          goal':term{Subst goal s2 (WithPrefix pref goal')} *
-                          infon':term{Subst infon s2 (WithPrefix pref infon')}))
-      : option (s3:substitution{Extends s3 s1} * 
-                  (s4:substitution{Extends s4 s3} -> 
-                    (goal_res:term{Subst goal s4 goal_res} * entails s k g goal_res))) = 
-
-    let (s2, pref, goal', infon') = arg in 
-    let mkpf_infon (s3:substitution{Extends s3 s2}) : 
-        (infon'':term{Subst infon' s3 infon''} * entails s k g infon'') = 
-      (match checkWF s k g with
-         | None -> raise "ill-formed environment"
-         | Some pf_wf -> (* this is P-kinded, I don't get it *)	    
-	     let infon'' = subst infon' s3 in 
-	       if (infon:term) = infon''
-	       then (infon'', 
-		     Entails_Hyp_Knowledge s k g infon pf_wf)
-	       else (* TODO: Must use Entails_Alpha to conclude *)
-                 raise "not a closed infon in infostrate") in
-      match tryDerive s k g u s2 pref goal' infon' mkpf_infon with 
-        | None -> None
-        | Some((s3, mkpf)) -> (* Extends s3 s2 *)
-            let mkpf_pair (s4:substitution{Extends s4 s3}) = 
-              let (goal'', pref', entails_pf) = mkpf s4 in 
-                (* Have:
-                      Subst goal' s4 goal'' 
-                      SubstList pref s4 pref' 
-                      entails s k g (WithPrefix pref' goal'') *)
-              let goal_res = withPrefix pref' goal'' in 
-              let s4_goal = subst goal s4 in 
-                (* Need: 
-                      goal_res : Subst goal s4 goal_res
-                      entails s k g goal_res *)
-                if (s4_goal : term) = goal_res 
-                then ((goal_res, entails_pf):
-                        (goal_res:term{Subst goal s4 goal_res} * entails s k g goal_res))
-                else raise "impos"
-                  (* TODO: Should be able to use this and q-free goal to conclude unreachable
-                     Subst goal s2 (WithPrefix pref goal') *) in 
-              Some (s3, mkpf_pair) in 
-  let prefixes = allSharedPrefixes u s1 goal infon in 
-    map_one prefixes callTryDerive 
-      
-
-(* result S K G s3 pref goal) *)
-and doDerive s k g u s1 pref goal = 
+let rec doDerive s k g u s1 pref goal =
   match goal with
-    | ForallT x i -> 
-        if not (pref = [])
-        then raise "impos"
-        else 
-          if containsVar g x 
-          then (* alpha convert first *)  None
-          else
-            (match doDerive s k (x::g) u s1 pref i with 
-               | None -> None
-               | Some ((s2, mkpf)) -> 
-                   let cont (s3:substitution{Extends s3 s2}) = 
-                     let (i', _, entails_i') = mkpf s3 in 
-                       (* Have: Subst i s3 i' 
-                          entails s k (x::g) i'
-                          
-                          Need: goal':term
-                          Subst (ForallT x i) s3 goal' 
-                          entails s k g goal' *)
-                     let goal' = ForallT x i' in 
-                       if contains x (freeVarsSubst s3)
-                       then raise "bad subst" (* TODO: carry invariant that (FreeVarsSubst s) disjoint from g *)
-                       else 
-                         let entails_goal' : entails s k g goal' =
-                           Entails_Q_Intro s k g x i' entails_i' in 
-                           ((goal', [], entails_goal') :
-                              (goal':term{Subst goal s3 goal'} *
-                                 pref':prefix{SubstList pref s3 pref'} *
-                                 entails s k g (WithPrefix pref' goal'))) in 
-                     Some (s2, cont))
-            
-    | App EmptyInfon [] -> 
-        let continuation (s2:substitution{Extends s2 s1}) =
-          let pref' = substList pref s2 in
-            match checkWF s k g, 
-              doType g (WithPrefix pref' (App EmptyInfon [])) with 
-                | Some pf_wf, Some((Infon, pf_typ)) ->
-                    ((goal, pref', Entails_Emp s k g pref' pf_wf pf_typ) :
-                       (goal':term{Subst goal s2 goal'} *
-                          pref':prefix{SubstList pref s2 pref'} *
-                          entails s k g (WithPrefix pref' goal')))
-                | None, _ -> raise "ill-formed environment"
-                | _, None -> raise "ill-typed term"
-        in Some(s1, continuation) 
+    | App EmptyInfon [] ->
+        let mkpf (s2:substitution{Extends s2 s1}) : kresult s k g pref goal s2 = 
+          let pref' = substList pref s2 in 
+          let goal' = withPrefix pref' (App EmptyInfon []) in 
+          let ty, pf_typing = doTyping g goal' in 
+            match ty with 
+              | Infon -> MkPartial (Entails_Emp s k g pref' pf_typing)
+              | _ -> raise "Unreachable" 
+        in Some(s1, mkpf)
 
-    | App AndInfon [goal_i; goal_j] -> 
-        (match doDerive s k g u s1 pref goal_i with 
+    | App AndInfon [goal_i; goal_j] ->
+        (match doDerive s k g u s1 pref goal_i with
            | None -> None
-           | Some((s2, mkpf_i)) -> 
-               match doDerive s k g u s2 pref goal_j with 
+           | Some((s2, mkpf_i)) ->
+               match doDerive s k g u s2 pref goal_j with
                  | None -> None
-                 | Some((s3, mkpf_j)) -> 
-                     let continuation (s4:substitution{Extends s4 s3}) = 
-                       let goal_i', pref_i', pf_i' = mkpf_i s4 in (* from lemma: Extends s4 s2 *) (* pf_i': entails s k g (WithPrefix pref_i' goal_i') *) 
-                       let goal_j', pref_j', pf_j' = mkpf_j s4 in (* Extends s4 s3, directly *) (* pf_j': entails s k g (WithPrefix pref_j' goal_j') *)
-                         if (pref_i'=pref_j') (* we know: Subst pref s4 pref_i' and  Subst pref s4 pref_j'; but not pref_i'=pref_j' *)
-                         then
-                           let pf_and = Entails_And_Intro2 s k g
-                             goal_i' goal_j' pref_i' pf_i' pf_j' in
-                           let goal' = App AndInfon [goal_i'; goal_j'] in  (* pf_and: Entails s k g goal'*)
-                             ((goal', pref_i', pf_and)
-                                :(goal':term{Subst goal s4 goal'} *
-                                    pref':prefix{SubstList pref s4 pref'} *
-                                    entails s k g (WithPrefix pref' goal')))
-                         else raise "bad substitution" in 
-                       Some (s3, continuation))
-          (*
-            | App AsInfon [SubstrateQueryTerm q] ->
-            (match pref with
-            | [] ->
-            (match check_substrate s q with
-            | false -> None
-            | true ->
-            let continuation (s2:substitution{Extends s2 s1}) =
-            let goal' = subst goal s2 in
-            match checkWF s k g, goal' with
-            | None, _ -> raise "ill-formed environment"
-            | Some pf_wf, App AsInfon [SubstrateQueryTerm q'] ->
-            let pf = Entails_Hyp_Substrate s k g q pf_wf in
-	  (* I want to conclude with goal', but I only have
-	    the proof of q, not the proof of goal' = AsInfon(q') *)
-	  (* This is (again) an instance of the substitution rule *)
-            let pref' = substList pref s2 in
-            ((goal', pref', pf) 
-            :(goal':term{Subst goal s2 goal'} *
-            pref':prefix{SubstList pref s2 pref'} *
-            entails s k g (WithPrefix pref' goal')))
-	    | _ -> raise "impos"
-            in
-            Some(s1, continuation) )
-            | _ -> raise "asInfon(...) under prefix")
-          *)
+                 | Some((s3, mkpf_j)) ->
+                     let mkpf (s4:substitution{Extends s4 s3}) : kresult s k g pref goal s4 = 
+                       match mkpf_i s4, mkpf_j s4 with (* from lemma: Extends s4 s2 *)
+                         | MkPartial pf_i, MkPartial pf_j -> (* pf_x : (entails s k g (Subst (WithPrefix pref goal_x) s4)) *)
+                             let pf_and = (Entails_And_Intro s k g 
+                                             (subst goal_i s4)
+                                             (subst goal_j s4)
+                                             (substList pref s4)
+                                             pf_i pf_j) in 
+                               MkPartial pf_and
+                     in Some (s3, mkpf))
+ 
     | App ImpliesInfon [goal_i; goal_j] ->
         (match doDerive s k g u s1 pref goal_j with
            | None -> None
            | Some((s2, mkpf_j)) ->
-               let continuation (s3:substitution{Extends s3 s2}) =
-                 let goal_j', pref_j', pf_j' = mkpf_j s3 in
-                 let goal_i' = subst goal_i s3 in
-                   match doType g goal_i' with
-                     | Some((Infon, pf_typ)) ->
-                         let pf_imp = Entails_W_Imp_Intro s k g 
-                           goal_i' goal_j' pref_j' pf_j' pf_typ in
-                         let goal' = App ImpliesInfon [goal_i'; goal_j'] in
-                           ((goal', pref_j', pf_imp)
-                              : (goal':term{Subst goal s3 goal'} *
-                                   pref':prefix{SubstList pref s3 pref'} *
-                                   entails s k g (WithPrefix pref' goal')))
-                     | None -> raise "ill-typed term" in
-                 Some (s2, continuation))
-          
-          
-    | App SaidInfon [p;j] ->
-        (match doDerive s k g u s1 (p::pref) j with
-           | Some ((s2, mkpf_j)) ->  (* s2:substitution{Extends s2 s1} * (s3:subst{Extends s3 s2} -> (goal_j':term{Subst goal_j s3 goal_j'} *
-                                        pref_j':prefix{SubstList (p::pref) s3 pref'} *
-                                        entails s k g (WithPrefix pref_j' goal_j'))) *)
-               let continuation (s3:substitution{Extends s3 s2}) =
-                 let goal_j', pref_j', pf_j' = mkpf_j s3 in (* SubstList (p::pref) s3 pref_j'; we should prove that pref_j' = p'::pref' where (Subst p s3 p') *)
-                   match pref_j' with
-                     | p'::pref' -> (* should prove that (Subst p s3 p') *)
-                         let goal' = App SaidInfon [p'; goal_j'] in
-                           ((goal', pref', pf_j')
-                              : (goal':term{Subst goal s3 goal'} * pref':prefix{SubstList pref s3 pref'} * entails s k g (WithPrefix pref' goal')))
-                     | [] -> raise "impos" in (* prove that this case is unreachable by asserting false *) 
-                 Some (s2, continuation))
-	  
-    | _ -> 
-        let pref_goal = withPrefix pref goal in 
-        let call_tryDerive (infon:term{In infon k}) 
-            : option (s2:substitution{Extends s2 s1} *
-                        (s3:substitution{Extends s3 s2} -> (goal':term{Subst goal s3 goal'} *
-                                                              pref':prefix{SubstList pref s3 pref'} *
-                                                              entails s k g (WithPrefix pref' goal')))) = 
-	  
-          match tryDeriveWrapper s k g u s1 pref_goal infon with 
-            | None -> None 
-            | Some ((s2, mk_pref_goal_pair)) -> 
-                let mk_pref_goal (s3:substitution{Extends s3 s2}) =
-                  let pref_goal', entails_pref_goal' = mk_pref_goal_pair s3 in 
-                    (* Subst pref_goal s3 pref_goal' *)
-                    (* entails s k g pref_goal' *)
-                    (* We know: pref_goal' = (s3 (WithPrefix pref goal)) *)
-                  let pref' = substList pref s3 in (* SubstList pref s3 pref' *)
-                  let goal' = subst goal s3 in 
-                  let goal'' = stripPrefix pref_goal' pref' in  
-                    (* entails s k g (WithPrefix pref' goal'') *)
-                    (* Need: Subst goal s3 goal' 
-                       and:  SubstList pref s3 pref'
-                       and:  entails s k g (WithPrefix pref' goal') *)
-                    if (goal' : term)=goal'' 
-                    then 
-                      ((goal', pref', entails_pref_goal'): 
-                         (goal':term{Subst goal s3 goal'} *
-                            pref':prefix{SubstList pref s3 pref'} *
-                            entails s k g (WithPrefix pref' goal')))
-                    else raise "Impos" (* TODO: if goal is q-free we're done *)  in 
-                  Some (s2, mk_pref_goal) in
-          map_one k call_tryDerive 
+               let mkpf (s3:substitution{Extends s3 s2}) : kresult s k g pref goal s3 = 
+                 match mkpf_j s3 with 
+                   | MkPartial pf_j -> 
+                       let goal_i' = subst goal_i s3 in
+                       match doTyping g goal_i' with 
+                         | (Infon, typing_i) -> 
+                             let pf_imp = (Entails_W_Imp_Intro s k g 
+                                             goal_i'
+                                             (subst goal_j s3) 
+                                             (substList pref s3) 
+                                             pf_j
+                                             typing_i) in 
+                               MkPartial pf_imp 
+                         | _ -> raise "Ill-typed formula"
+               in Some (s2, mkpf))
 
-(* with (\* should this be done last? *\) *)
-(*           | Some result -> Some result *)
-(*           | None -> None *)
+    | App SaidInfon [p;j] -> 
+        (match doDerive s k g u s1 (p::pref) j with (* Ugly---expansion necessary because of no structural subtyping on tuples? *)
+           | None -> None
+           | Some ((s2, mkpf_j)) -> Some (s2, mkpf_j))
+               
+    | App AsInfon [SubstrateQueryTerm q] ->
+        (match pref with
+           | [] -> 
+               let mkpf (s2:substitution{Extends s2 s1}) : kresult s k g pref goal s2 =
+                 let q' = substQuery q s2 in
+                   if check_substrate s q'
+                   then MkPartial (Entails_Hyp_Substrate s k g q')
+                   else raise "Substrate query failed" 
+               in Some (s1, mkpf)
+           | _ -> None) (* AsInfon not allowed under prefix *)
+	  
+    | _ -> map_one k (tryDeriveAlpha s k g u s1 pref goal)
+
+and tryDeriveAlpha s k g u s1 pref goal infon = 
+  let infon', aeq = alphaConvert infon in 
+    match doPolyTyping [] infon, doPolyTyping g infon' with 
+      | MkPartial typing_infon, MkPartial typing_infon' -> 
+          let mkpf (s2:substitution{Extends s2 s1}) : kpolyresult s k g infon' s2 = 
+            match infon' with 
+              | ForallT xs body -> 
+                  if check_disjoint (freeVarsSubst s2) xs
+                  then 
+                    let body' = subst body s2 in 
+                      if body = body'
+                      then MkPartial (Entails_Hyp_Knowledge s k g infon infon' typing_infon aeq typing_infon')
+                      else raise "TODO: prove using Domain(s2) = u, disjoint from (g \union xs)=Vars body"
+                  else raise "Substitution domain"
+                    
+              | MonoTerm body -> 
+                  let body' = subst body s2 in 
+                    if body = body'
+                    then MkPartial (Entails_Hyp_Knowledge s k g infon infon' typing_infon aeq typing_infon') 
+                    else raise "TODO: prove using Domain(s2) = u, disjoint from (g \union xs)=Vars body"
+          in 
+            tryDerive s k g u s1 pref goal infon' mkpf
+
+and tryDerive s k g u s1 pref goal infon mkpf_infon = 
+  match infon with
+    | ForallT xs body -> 
+        let pref_goal = withPrefix pref goal in 
+        (match unify s1 u xs body pref_goal with
+           | None -> None 
+           | Some((s2, insts)) -> 
+               let mkpf (s3:substitution{Extends s3 s2}) : kresult s k g pref goal s3 = 
+                 let insts = map (fun i -> subst i s3) insts in 
+                   if not (check_disjoint (freeVarsSubst s3) xs)
+                   then raise "TODO: Substitution domain" 
+                   else
+                     match doTypingList g insts xs, mkpf_infon s3 with
+                       | None, _ -> raise "Ill-typed unification"
+                       | Some typing_insts, MkPartial pf_infon -> 
+                           let sinst = mkSubst xs insts in 
+                           let body' = subst (subst body s3) sinst in 
+                           let pref_goal' = subst pref_goal s3 in 
+                             if (pref_goal':term)=body' 
+                             then MkPartial (Entails_Q_Elim s k g xs (subst body s3) insts pf_infon typing_insts)
+                             else raise "Unification error" (* TODO: prove unification correct *)
+               in Some (s2, mkpf))
+          
+    | MonoTerm (App AndInfon [infon1; infon2]) ->
+        let monoinfon = App AndInfon [infon1; infon2] in
+        let mkpf_infon1 (s4:substitution{Extends s4 s1}) : kpolyresult s k g (MonoTerm infon1) s4 = 
+          match mkpf_infon s4 with 
+            | MkPartial pf_infon ->
+                MkPartial (Entails_Mono s k g (subst infon1 s4)
+                             (Entails_And_Elim1 s k g (subst infon1 s4) (subst infon2 s4) [] 
+                                (Entails_Poly s k g (subst monoinfon s4) pf_infon))) in
+        let mkpf_infon2 (s4:substitution{Extends s4 s1}) : kpolyresult s k g (MonoTerm infon2) s4 = 
+          match mkpf_infon s4 with 
+            | MkPartial pf_infon ->
+                MkPartial (Entails_Mono s k g (subst infon2 s4)
+                             (Entails_And_Elim2 s k g (subst infon1 s4) (subst infon2 s4) [] 
+                                (Entails_Poly s k g (subst monoinfon s4) pf_infon))) in
+          (match tryDerive s k g u s1 pref goal (MonoTerm infon1) mkpf_infon1 with
+             | Some res -> Some res
+             | None -> tryDerive s k g u s1 pref goal (MonoTerm infon2) mkpf_infon2)
             
+    | MonoTerm (App ImpliesInfon [i; j]) ->
+        let monoinfon = App ImpliesInfon [i; j] in
+          (match doDerive s k g u s1 [] i with (* TODO: This is no longer backwards chaining. Fix. *)
+             | None -> None
+             | Some((s2, mkpf_i)) ->
+                 let mkpf_j (s4:substitution{Extends s4 s2}) : kpolyresult s k g (MonoTerm j) s4 = 
+                   match mkpf_infon s4, mkpf_i s4 with 
+                     | MkPartial pf_infon, MkPartial pf_i -> 
+                         MkPartial (Entails_Mono s k g (subst j s4)
+                                      (Entails_Imp_Elim s k g 
+                                         (subst i s4) (subst j s4) [] 
+                                         pf_i 
+                                         (Entails_Poly s k g (subst monoinfon s4) pf_infon)))
+                 in 
+                   match tryDerive s k g u s2 pref goal (MonoTerm j) mkpf_j with
+                     | None -> None
+                     | Some ((s3, mkpf)) -> Some (s3, mkpf)) (* Need to repack the existential at a different type *)
+
+  | MonoTerm i -> 
+      let pref_goal = withPrefix pref goal in
+        match unify s1 u [] i pref_goal with
+          | Some ((s2,[])) ->
+              let mkpf (s3:substitution{Extends s3 s2}) : kresult s k g pref goal s3 =
+                match mkpf_infon s3 with
+                  | MkPartial pf_infon ->
+                      let i' = subst i s3 in 
+                      if (i':term) = (subst pref_goal s3)
+                      then MkPartial (Entails_Poly s k g i' pf_infon)
+                      else raise "Unification error" 
+              in Some (s2, mkpf)
+          | _ -> None
+
+val deriveQuant: U:vars             (* Variables available for unification in goal (free in goal) *)
+              -> S:substrate 
+              -> K:infostrate 
+              -> G:vars
+              -> goal:term
+              -> option (s:substitution(* {(Domain s)=U} *) *
+                         polyentails S K [] (ForallT G (Subst goal s)))
+let rec deriveQuant u s k g goal = 
+  match decideWFG g with 
+    | None -> None
+    | Some wfg -> 
+        let s0 = emptySubst() in 
+          match doDerive s k g u s0 [] goal with 
+            | None -> None
+            | Some ((s1, mkpf)) -> 
+                match mkpf s1 with 
+                  | MkPartial pfs1 -> 
+                      let res = Entails_Q_Intro s k g (subst goal s1) wfg pfs1 in 
+                        Some ((s1, res))
+                  | _ -> None
