ModularEngine/src/LogicEngine.FStar/subst.fst
@@ -3,69 +3,70 @@ open Types
 open Util
 
 (* Axiomatization of sets of variables *)
-logic function Empty : varset
-logic function Singleton : var -> varset
-logic function Union : varset -> varset -> varset
+logic function Empty : vars
+logic function Singleton : var -> vars
+logic function Union : vars -> vars -> vars
 assume forall (v:var). (In v (Singleton v))
-assume forall (l1:varset) (l2:varset) (v:var). 
+assume forall (l1:vars) (l2:vars) (v:var). 
         ((In v l1) || (In v l2)) <=> (In v (Union l1 l2))
 assume forall (v:var). not(In v Empty)
-(* extern Runtime *) val union : s1:varset -> s2:varset -> s3:varset{(s3 = (Union s1 s2))}
 
 (* Axiomatization of substitutions *)
-logic function EmptySubst : substitution
-logic function Domain : substitution -> varset
 logic function Select : substitution -> var -> term
 logic function Update : substitution -> var -> term -> substitution
-logic function FreeVars : term -> varset
-logic function FreeVarsSubst : substitution -> varset 
-  (* set of variable in both the domain and the range of the map *)
-assume forall (s:substitution) (x:var) (t:term). 
-  (Select (Update s x t) x) = t
-assume forall (s:substitution) (x:var) (y:var) (t:term).
-  (x <> y) => ((Select (Update s x t) y) = (Select s y))
-assume forall (s:substitution) (x:var) (t:term). 
-  Domain (Update s x t) = (Union (Domain s) (Singleton x))
+assume forall (s:substitution) (x:var) (t:term). (Select (Update s x t) x) = t
+assume forall (s:substitution) (x:var) (y:var) (t:term). (x <> y) => ((Select (Update s x t) y) = (Select s y))
+
+(* Domain of a substitution will be restricted to be a subset of the unification variables *)
+logic function Domain : substitution -> vars
+logic function EmptySubst : substitution
+assume forall (s:substitution) (x:var) (t:term). Domain (Update s x t) = (Union (Domain s) (Singleton x))
 assume (Domain EmptySubst) = Empty
 
-type Subst :: term => substitution => term => E
-type SubstList :: list term => substitution => list term => E
+(* freevars of both the domain and the range *)
+logic function FreeVars : term -> vars
+logic function FreeVarsSubst : substitution -> vars 
 
+
+(* Axiomatization of substitution itself *)
+logic function SubstQuery : ISubstrateQueryTerm -> substitution -> ISubstrateQueryTerm
+logic function Subst : term -> substitution -> term
+logic function SubstList : list term -> substitution -> list term
 assume Subst_VarRepl: forall (x:var) (s:substitution).
-        (In x (Domain s)) => ((Subst (Var x) s (Select s x)))
+        (In x (Domain s)) => ((Subst (Var x) s)=(Select s x))
 assume Subst_VarIgnore: forall (x:var) (s:substitution).
-        (not (In x (Domain s))) => (Subst (Var x) s (Var x))
-assume Subst_Const:  (forall (c:constant) (s:substitution). 
-        (Subst (Const c) s (Const c)))
-assume Subst_App: forall (f:func) (args:list term) (args': list term) (s:substitution).
-        (SubstList args s args') =>  (Subst (App f args) s (App f args'))
-assume Subst_forallT: forall (x:var) (t:term) (s:substitution) (t':term). 
-        (not(In x (FreeVarsSubst s)) && Subst t s t') => 
-           (Subst (ForallT x t) s (ForallT x t'))
-assume Subst_forallT_Alpha: forall (x:var) (t:term) (s:substitution) (y:var) (t_yx:term) (t':term). 
-        (not(In y (Union (FreeVarsSubst s) (FreeVars t))) &&
-            (Subst t (Update EmptySubst x (Var y)) t_yx) &&
-            (Subst t_yx s t'))
-        => (Subst (ForallT x t) s (ForallT y t'))
+        (not (In x (Domain s))) => ((Subst (Var x) s)=(Var x))
+assume Subst_Const: forall (c:constant) (s:substitution). 
+        (Subst (Const c) s)=(Const c)
+assume Subst_App: forall (f:func) (args:list term) (s:substitution).
+          ((Subst (App f args) s)=(App f (SubstList args s)))
+assume Subst_QueryTerm: forall (q:ISubstrateQueryTerm) (s:substitution). 
+          ((Subst (SubstrateQueryTerm q) s)=(SubstrateQueryTerm (SubstQuery q s)))
+assume SubstList_nil: forall (s:substitution). ((SubstList [] s)=[])
+assume SubstList_cons: forall (t:term) (tl:list term) (s:substitution). 
+           (SubstList (t::tl) s) = ((Subst t s)::(SubstList tl s))
 
-assume SubstList_nil: forall (s:substitution). (SubstList [] s [])
-assume SubstList_nil_inv_x: forall (s:substitution) (x:list term). 
-     (SubstList x s []) => (x=[])
-assume SubstList_nil_inv_y: forall (s:substitution) (y:list term). 
-     (SubstList [] s y) => (y=[])
-assume SubstList_cons: forall (t:term) (t':term) (tl:list term) (tl':list term) (s:substitution). 
-        (Subst t s t' && SubstList tl s tl')
-    <=> (SubstList (t::tl) s (t'::tl'))
+logic function PolySubst : polyterm -> substitution -> polyterm
+assume (forall (s:substitution) (xs:vars) (body:term). Disjoint (FreeVarsSubst s) xs =>
+    ((PolySubst (ForallT xs body) s)=(ForallT xs (Subst body s))))
+assume (forall (s:substitution) (body:term). 
+    ((PolySubst (MonoTerm body) s)=(MonoTerm (Subst body s))))
+
+(* Building substitutions *)
+logic function MkSubst: vars -> list term -> substitution
+assume (MkSubst [] [] = EmptySubst)
+assume (forall (x:var) (t:term) (xs:vars) (ts:list term). (MkSubst (x::xs) (t::ts)) = (Update (MkSubst xs ts) x t))
+(* extern *) val mkSubst : xs:vars -> ts:list term -> s:substitution{s=(MkSubst xs ts)}
 
 
 type Extends :: substitution => substitution => E
 assume forall (s:substitution). Extends s s
 assume forall (s1:substitution) (s2:substitution) (x:var) (t:term). 
-          ((Extends s2 s1) && (Subst t s2 t) && (not(In x (Domain s2))))
+          ((Extends s2 s1) && ((Subst t s2)=t) && (not(In x (Domain s2))))
         => Extends (Update s2 x t) s1
 
-
-val emptySubst: unit -> s:substitution{s=EmptySubst}
+(* extern *) val substQuery: q:ISubstrateQueryTerm -> s:substitution -> q':ISubstrateQueryTerm{(SubstQuery q s)=q'}
+(* extern *) val emptySubst: unit -> s:substitution{s=EmptySubst}
   
 val lookupVar : 
      s:substitution 
@@ -77,7 +78,7 @@ val lookupVar :
 val extendSubst : 
      s:substitution 
   -> x:var 
-  -> t:term{Subst t s t && not(In x (Domain s))}
+  -> t:term{(Subst t s)=t && not(In x (Domain s))}
   -> s':substitution{s'=(Update s x t)}
 
 val inDomain : 
@@ -90,90 +91,53 @@ val inFreevars :
   -> x:var 
   -> b:bool{b=true <=> In x (FreeVarsSubst s)}
 
-(* added *)
 val freeVarsSubst : 
      s:substitution 
-  -> f:varset{(f = (FreeVarsSubst s))}
+  -> f:vars{(f = (FreeVarsSubst s))}
 
 val freeVars : 
      t:term 
-  -> f:varset{(f = (FreeVars t))}
+  -> f:vars{(f = (FreeVars t))}
 
+let genId =
+  let ctr = ref 0 in 
+    fun (x:unit) -> 
+      (ctr := !ctr + 1); 
+      !ctr
 
-(* functions from builders.fs *)
-let _freshVarId = ref 0 (* can't go inside because no inside rec function *)
+val freshVar : ty:typ -> x:var{x.typ=ty}
+let freshVar ty = { typ = ty; name = (Concat "__fresh" (string_of_any (genId())))}
 
-val freshVar : ty:typ -> s:varset 
-             -> x:var{ not ( In x s ) }
-let rec freshVar ty s =
-  let n = { typ = ty; name = (Concat "fresh" (string_of_any (!_freshVarId))) } in
-   (_freshVarId := !_freshVarId + 1); (* Rk: parenthesis needed *)
-   if not (contains n s) 
-   then n 
-   else freshVar ty s
-     
-(* from term.fst *)	 
-extern reference TranslationToFStar {language="F#";
-                                     dll="TranslationToFStar";
-                                     namespace="";
-                                     classname="TranslationToFStar"}
-extern TranslationToFStar val FStarVarOfIVar : IVar -> Types.var
-extern TranslationToFStar val FStarTermOfITerm : ITerm -> Types.term
-extern TranslationToFStar val FStarSubstitutionOfISubstitution: ISubstitution -> Types.substitution	 
-	 
+type varTyEq :: _ = (fun (x:var) (y:var) => (x.typ=y.typ))
+type varsTyEq :: _ = (fun (xs:vars) (ys:vars) => (ZipE var var varTyEq xs ys))
+val freshVars: xs:vars -> (ys:vars * varsTyEq xs ys)
+let rec freshVars xs = match xs with 
+  | [] -> ([], ZipE_Nil<var, var, varTyEq>)
+  | x::xtl -> 
+      let y = freshVar x.typ in 
+      let ytl, ztl = freshVars xtl in 
+        ((y::ytl), ZipE_Cons<var,var,varTyEq> xtl ytl x y ztl)
+
+  
 (* see term_apply in term.fst *)
-val subst: i:term -> s:substitution -> i':term{Subst i s i'}
-val substList : tl:list term -> s:substitution -> tl':list term{SubstList tl s tl'}
-let rec subst i s = 
-  match i with
-    | Var y -> 
-        (match lookupVar s y with 
-           | None -> Var y
-           | Some t -> t)
-          
-    | Const c -> Const c
-        
-    | App f tl -> App f (substList tl s)
-    
-    | ForallT x t -> (* code taken partially from term.fst *)
-      (* the substitution is not applied to the quantified variable *)
-        let y : (yy:var{not(In yy (Union (FreeVars t) (FreeVarsSubst s)))}) =
-          freshVar x.typ (union (freeVars t) (freeVarsSubst s)) in
-		let ySubst : (ys:substitution{(ys = (Update EmptySubst x (Var y)))}) =
-          extendSubst (emptySubst ()) x (Var y) in
-		let t_yx : (t_yx:term{((Subst t (Update EmptySubst x (Var y)) t_yx))}) =
-          subst t ySubst in
-		let t' : (t':term{(Subst t_yx s t')}) =
-          (subst t_yx s) in
-(*         let res : (res:term{Subst i s res}) = Types.ForallT y t' in  *)
-        let res = Types.ForallT y t' in 
-	let _ = Assume <(Subst i s res)> () in
-		res
-		
-(*     | SubstrateQueryTerm t0 -> *)
-(* 	    let res =  *)
-(*           FStarTermOfITerm *)
-(*             (TypeHeaders.substrateQueryTerm_apply t0   *)
-(* 		       (\* not sure why I need the TypeHeaders. , TypeHeaders has been opened *\) *)
-(* 		       (TranslationFromFStar.ISubstitutionOfFStarSubstitution s) ) *)
-(* 		in let _ = Assume <(res = (Subst i s))> () in *)
-(* 		res *)
+(* NS: Would be nice to have this be the only definition of subst 
+       and generate the logic function axioms from this code. *)
+val subst: i:term -> s:substitution -> i':term{(Subst i s)=i'}
+val substList : tl:list term -> s:substitution -> tl':list term{(SubstList tl s)=tl'}
+let rec subst i s = match i with
+  | Var y -> (match lookupVar s y with 
+                | None -> Var y
+                | Some t -> t)
+  | Const c -> Const c
+  | App f tl -> App f (substList tl s)
+  | SubstrateQueryTerm q ->
+      let q' = substQuery q s in 
+        SubstrateQueryTerm q'
 	
-(*     | SubstrateUpdateTerm t0 -> *)
-(* 	    let res = *)
-(*           FStarTermOfITerm  *)
-(*             (TypeHeaders.substrateUpdateTerm_apply t0  *)
-(* 		       (TranslationFromFStar.ISubstitutionOfFStarSubstitution s) ) *)
-(* 		in let _ = Assume <(res = (Subst i s))> () in *)
-(* 		res *)
-	
-(*     | ConcretizationEvidence t1 s1 -> raise "Evidences not handled" *)
-(* 	  (\* ConcretizationEvidence (ConcretizationEvidence t1 s1) s *\) (\* correct?? *\) *)
-(*       (\* Types.ConcretizationEvidence t1 (composeWith s s1) *\) *)
-
 and substList ilist s = match ilist with
   | [] -> []
   | hd::tl -> 
       let tl' = substList tl s in 
       let hd' = subst hd s in
-        Cons<term>  hd' tl' (* type inference is too eager here; need to provide explicit annotation on Cons *)
+        Cons<term> hd' tl' (* type inference is too eager here and infers a refined instantiation; 
+                              need to provide explicit annotation on Cons *)
