ModularEngine/src/LogicEngine.FStar/util.fst
@@ -1,12 +1,6 @@
 module Util
 open Types
 
-type substrate
-type infostrate = list term
-type varDecl = list var
-type prefix = list term
-type varset = list var
-
 (*************)
 (* Utilities *)
 (*************)
@@ -24,9 +18,6 @@ let rec mem (a : 'a) (l: list 'a) : option (Mem 'a a l) =
                | None -> None
                | Some(m) -> Some(Mem_tl a h t m))
 			   
-val contains : a:'a -> l:list 'a -> b:bool{((b=true) <=> (In 'a a l))}
-
-
 val fold_left_dep : res:'a -> l:list 'b -> ('a -> x:'b -> Mem x l -> 'a) -> 'a
 let rec fold_left_dep res l f = match l with
   | [] -> res
@@ -80,6 +71,16 @@ let rec mapL_p f l = match l with
 	   | Some pf_tl, Some pf_hd ->
 	       Some (MapL_Cons<'a,'Q> t h pf_tl pf_hd)
 	   | _ -> None
+
+type ZipE :: 'a::* => 'b::* => ('a => 'b => E) => list 'a => list 'b => P = 
+   | ZipE_Nil : 'a::* -> 'b::* -> 'Q::('a => 'b => E) 
+             -> ZipE 'a 'b 'Q [] []
+   | ZipE_Cons: 'a::* -> 'b::* -> 'Q::('a => 'b => E)
+             -> l1:list 'a -> l2:list 'b 
+             -> x:'a -> y:'b{'Q x y}
+             -> ZipE 'a 'b 'Q l1 l2
+             -> ZipE 'a 'b 'Q (x::l1) (Cons<'b> y l2)
+
 
 type Zip :: 'a::* => 'b::* => ('a => 'b => P) => list 'a => list 'b => P = 
    | Zip_Nil : 'a::* -> 'b::* -> 'Q::('a => 'b => P) 
@@ -142,3 +143,14 @@ let rec map_mapL_p f l = match l with
                   MapL_Cons<'b, 'R> t' h' rt rh))
 	    | _ -> None)
 
+type Partial :: P => * = 
+  | MkPartial : 'a::P -> 'a -> Partial 'a
+
+logic function lconcat : list 'a -> list 'a -> list 'a
+assume (forall (x:list 'a). (lconcat [] x) = x)
+assume (forall (hd:'a) (tl:list 'a) (x:list 'a). (lconcat (hd::tl) x) = (hd::(lconcat tl x)))
+
+val concat: l1:list 'a -> l2:list 'a -> l3:list 'a{l3=(lconcat l1 l2)}
+let rec concat l1 l2 = match l1 with 
+  | [] -> l2
+  | hd::tl -> hd::(concat tl l2)
